src/axiomatic/TsoSimLocal.v
@@ -380,3 +380,54 @@ Proof.
   - inv H1. inv H0. inv H1. inv LABEL. rewrite EID in EID0. inv EID0. ss.
   - inv H1. ss. subst. eapply FWDN. econs; eauto. econs; eauto with tso.
 Qed.
+
+Definition sim_local_lper ex loc :=
+  (⦗ex.(Execution.label_is) (Label.is_kinda_writing loc)⦘ ⨾ (Execution.rfe ex)^? ⨾
+   Execution.po ⨾
+   ⦗ex.(Execution.label_is) (Label.is_flushopting loc)⦘ ⨾
+   Execution.po) ∪
+
+  (⦗ex.(Execution.label_is) (Label.is_kinda_read)⦘ ⨾
+   Execution.po ⨾
+   ⦗ex.(Execution.label_is) (Label.is_flushopting loc)⦘ ⨾
+   Execution.po) ∪
+
+  (⦗ex.(Execution.label_is) Label.is_access⦘ ⨾
+   Execution.po ⨾
+   ⦗ex.(Execution.label_is) (Label.is_barrier_c Barrier.is_dmb_dsb_wr)⦘ ⨾
+   Execution.po ⨾
+   ⦗ex.(Execution.label_is) (Label.is_flushopting loc)⦘ ⨾
+   Execution.po).
+
+Lemma sim_local_lper_step ex loc:
+  sim_local_lper ex loc =
+  (sim_local_lper ex loc ∪
+   ((⦗ex.(Execution.label_is) (Label.is_kinda_writing loc)⦘ ⨾ (Execution.rfe ex)^? ⨾
+      Execution.po ⨾
+      ⦗ex.(Execution.label_is) (Label.is_flushopting loc)⦘) ∪
+
+    (⦗ex.(Execution.label_is) (Label.is_kinda_read)⦘ ⨾
+      Execution.po ⨾
+      ⦗ex.(Execution.label_is) (Label.is_flushopting loc)⦘) ∪
+
+    (⦗ex.(Execution.label_is) Label.is_access⦘ ⨾
+      Execution.po ⨾
+      ⦗ex.(Execution.label_is) (Label.is_barrier_c Barrier.is_dmb_dsb_wr)⦘ ⨾
+      Execution.po ⨾
+      ⦗ex.(Execution.label_is) (Label.is_flushopting loc)⦘))) ⨾
+  Execution.po_adj.
+Proof.
+  unfold sim_local_lper. rewrite ? (union_seq' Execution.po_adj), ? seq_assoc, ? union_assoc.
+  rewrite Execution.po_po_adj at 2 4 7.
+  rewrite (clos_refl_union Execution.po), union_seq, eq_seq.
+  rewrite ? (seq_union' (Execution.po ⨾ Execution.po_adj) Execution.po_adj), ? seq_assoc, ? union_assoc.
+  funext. i. funext. i. propext. econs; i.
+  - repeat match goal with
+           | [H: (_ ∪ _) _ _ |- _] => inv H
+           end;
+      eauto 10 using union_l, union_r.
+  - repeat match goal with
+           | [H: (_ ∪ _) _ _ |- _] => inv H
+           end;
+      eauto 10 using union_l, union_r.
+Qed.
